theories/Operational/Common/OSSchedulerViewContract.v
@@ -1,0 +1,469 @@
+From Stdlib Require Import List Arith.PeanoNat Lia Compare_dec.
+Import ListNotations.
+From RocqSched Require Import Foundation.Base.
+From RocqSched Require Import Semantics.Schedule.
+From RocqSched Require Import Semantics.ScheduleLemmas.ScheduleFacts.
+From RocqSched Require Import Multicore.Common.MultiCoreBase.
+From RocqSched Require Import Multicore.Common.Admissibility.
+From RocqSched Require Import Operational.Common.State.
+From RocqSched Require Import Operational.Common.Step.
+From RocqSched Require Import Operational.Common.Invariants.
+From RocqSched Require Import Operational.Common.StepLemmas.
+From RocqSched Require Import Operational.Common.OSProjectionInterface.
+From RocqSched Require Import Operational.Common.ConcreteExecution.
+From RocqSched Require Import Operational.Common.Projection.
+From RocqSched Require Import Operational.Common.OSLocalAdapterContract.
+From RocqSched Require Import Operational.Common.OSCausalityContract.
+
+Definition op_job_visible (m : nat) (st : OpState) (j : JobId) : Prop :=
+  (exists c, c < m /\ op_current st c = Some j) \/
+  In j (op_runnable st) \/
+  exists c, c < m /\ op_dispatch_target st c = Some j.
+
+Lemma released_monotone :
+  forall jobs j t1 t2,
+    t1 <= t2 ->
+    released jobs j t1 ->
+    released jobs j t2.
+Proof.
+  intros jobs j t1 t2 Hle Hrel.
+  unfold released in *.
+  lia.
+Qed.
+
+Lemma projected_job_not_running_if_runnable :
+  forall m st j t,
+    op_struct_inv m st ->
+    In j (op_runnable st) ->
+    ~ running m (project_schedule (fun _ => st)) j t.
+Proof.
+  intros m st j t Hinv Hin [c [Hlt Hrun]].
+  destruct Hinv as [_ _ Hnotin _ _].
+  apply (Hnotin c j Hrun).
+  exact Hin.
+Qed.
+
+Lemma projected_trace_job_not_running_if_runnable :
+  forall m tr j t,
+    op_struct_inv m (tr t) ->
+    In j (op_runnable (tr t)) ->
+    ~ running m (project_schedule tr) j t.
+Proof.
+  intros m tr j t Hinv Hin.
+  unfold running, project_schedule.
+  intros [c [Hlt Hrun]].
+  destruct Hinv as [_ _ Hnotin _ _].
+  apply (Hnotin c j Hrun).
+  exact Hin.
+Qed.
+
+Lemma visible_job_not_completed_if_not_running_next :
+  forall jobs m sched j t,
+    ~ completed jobs m sched j t ->
+    ~ running m sched j t ->
+    ~ completed jobs m sched j (S t).
+Proof.
+  intros jobs m sched j t Hncomp Hnotrun HcompS.
+  apply (proj1 (not_completed_iff_service_lt_cost jobs m sched j t)) in Hncomp.
+  apply (proj1 (completed_iff_service_ge_cost jobs m sched j (S t))) in HcompS.
+  rewrite service_job_no_increase_if_not_executed in HcompS.
+  - lia.
+  - intros c Hlt Hcur.
+    apply Hnotrun.
+    exists c. split; assumption.
+Qed.
+
+Record labeled_concrete_scheduler_view_contract
+    {CState : Type}
+    {P : OSLabeledProjection CState}
+    (jobs : JobId -> Job)
+    (m : nat)
+    (ex : labeled_concrete_execution P m) : Prop :=
+  mkLabeledConcreteSchedulerViewContract {
+    lcsv_visible_released :
+      forall t j,
+        op_job_visible
+          m
+          (os_to_op_state (osl_to_os_projection P) (lce_trace ex t))
+          j ->
+        released jobs j t;
+    lcsv_visible_not_completed :
+      forall t j,
+        op_job_visible
+          m
+          (os_to_op_state (osl_to_os_projection P) (lce_trace ex t))
+          j ->
+        ~ completed
+            jobs
+            m
+            (project_schedule (osl_to_op_trace P (lce_trace ex)))
+            j t;
+    lcsv_wakeup_visible :
+      forall t j,
+        os_step_label P (lce_trace ex t) (lce_trace ex (S t)) = EvWakeup j ->
+        op_job_visible
+          m
+          (os_to_op_state (osl_to_os_projection P) (lce_trace ex (S t)))
+          j;
+    lcsv_choose_visible :
+      forall t c j,
+        c < m ->
+        os_step_label P (lce_trace ex t) (lce_trace ex (S t)) = EvChoose c j ->
+        op_job_visible
+          m
+          (os_to_op_state (osl_to_os_projection P) (lce_trace ex (S t)))
+          j;
+    lcsv_dispatch_visible :
+      forall t c j,
+        c < m ->
+        os_step_label P (lce_trace ex t) (lce_trace ex (S t)) = EvDispatch c j ->
+        op_job_visible
+          m
+          (os_to_op_state (osl_to_os_projection P) (lce_trace ex (S t)))
+          j;
+    lcsv_preempt_old_visible :
+      forall t c old new,
+        c < m ->
+        os_step_label P (lce_trace ex t) (lce_trace ex (S t)) =
+        EvPreempt c old new ->
+        op_job_visible
+          m
+          (os_to_op_state (osl_to_os_projection P) (lce_trace ex (S t)))
+          old;
+    lcsv_preempt_new_visible :
+      forall t c old new,
+        c < m ->
+        os_step_label P (lce_trace ex t) (lce_trace ex (S t)) =
+        EvPreempt c old new ->
+        op_job_visible
+          m
+          (os_to_op_state (osl_to_os_projection P) (lce_trace ex (S t)))
+          new;
+    lcsv_block_clears_current :
+      forall t c j,
+        os_step_label P (lce_trace ex t) (lce_trace ex (S t)) = EvBlock j ->
+        op_current
+          (os_to_op_state (osl_to_os_projection P) (lce_trace ex (S t)))
+          c <> Some j;
+    lcsv_block_clears_runnable :
+      forall t j,
+        os_step_label P (lce_trace ex t) (lce_trace ex (S t)) = EvBlock j ->
+        ~ In j
+             (op_runnable
+                (os_to_op_state (osl_to_os_projection P) (lce_trace ex (S t))));
+    lcsv_block_clears_dispatch_target :
+      forall t c j,
+        c < m ->
+        os_step_label P (lce_trace ex t) (lce_trace ex (S t)) = EvBlock j ->
+        op_dispatch_target
+          (os_to_op_state (osl_to_os_projection P) (lce_trace ex (S t)))
+          c <> Some j;
+    lcsv_complete_sets_completed :
+      forall t j,
+        os_step_label P (lce_trace ex t) (lce_trace ex (S t)) = EvComplete j ->
+        completed
+          jobs
+          m
+          (project_schedule (osl_to_op_trace P (lce_trace ex)))
+          j (S t);
+    lcsv_complete_clears_current :
+      forall t c j,
+        os_step_label P (lce_trace ex t) (lce_trace ex (S t)) = EvComplete j ->
+        op_current
+          (os_to_op_state (osl_to_os_projection P) (lce_trace ex (S t)))
+          c <> Some j;
+    lcsv_complete_clears_runnable :
+      forall t j,
+        os_step_label P (lce_trace ex t) (lce_trace ex (S t)) = EvComplete j ->
+        ~ In j
+             (op_runnable
+                (os_to_op_state (osl_to_os_projection P) (lce_trace ex (S t))));
+    lcsv_complete_clears_dispatch_target :
+      forall t c j,
+        c < m ->
+        os_step_label P (lce_trace ex t) (lce_trace ex (S t)) = EvComplete j ->
+        op_dispatch_target
+          (os_to_op_state (osl_to_os_projection P) (lce_trace ex (S t)))
+          c <> Some j;
+  }.
+
+Arguments lcsv_visible_released
+  {CState P jobs m ex} _ _ _ _.
+Arguments lcsv_visible_not_completed
+  {CState P jobs m ex} _ _ _ _.
+Arguments lcsv_wakeup_visible
+  {CState P jobs m ex} _ _ _ _.
+Arguments lcsv_choose_visible
+  {CState P jobs m ex} _ _ _ _ _ _.
+Arguments lcsv_dispatch_visible
+  {CState P jobs m ex} _ _ _ _ _ _.
+Arguments lcsv_preempt_old_visible
+  {CState P jobs m ex} _ _ _ _ _ _ _.
+Arguments lcsv_preempt_new_visible
+  {CState P jobs m ex} _ _ _ _ _ _ _.
+Arguments lcsv_block_clears_current
+  {CState P jobs m ex} _ _ _ _ _.
+Arguments lcsv_block_clears_runnable
+  {CState P jobs m ex} _ _ _ _.
+Arguments lcsv_block_clears_dispatch_target
+  {CState P jobs m ex} _ _ _ _ _.
+Arguments lcsv_complete_sets_completed
+  {CState P jobs m ex} _ _ _ _.
+Arguments lcsv_complete_clears_current
+  {CState P jobs m ex} _ _ _ _ _.
+Arguments lcsv_complete_clears_runnable
+  {CState P jobs m ex} _ _ _ _.
+Arguments lcsv_complete_clears_dispatch_target
+  {CState P jobs m ex} _ _ _ _ _.
+
+Lemma local_labeled_concrete_projection_sound_current_released :
+  forall CState (P : OSLabeledProjection CState) jobs m
+         (ex : labeled_concrete_execution P m),
+    local_labeled_concrete_projection_sound jobs m ex ->
+    forall t c j,
+      c < m ->
+      op_current
+        (os_to_op_state (osl_to_os_projection P) (lce_trace ex t))
+        c = Some j ->
+      released jobs j t.
+Proof.
+  intros CState P jobs m ex Hlocal.
+  induction t as [|t IH]; intros c j Hlt Hrun.
+  - exact (llcps_init_release Hlocal c j Hlt Hrun).
+  - destruct (llcps_current_origin Hlocal t c j Hlt Hrun) as [Hprev | [Hdispatch | Hpreempt]].
+    + exact (released_monotone jobs j t (S t) (Nat.le_succ_diag_r t) (IH c j Hlt Hprev)).
+    + exact (llcps_dispatch_release Hlocal t c j Hlt Hdispatch).
+    + destruct Hpreempt as [old Hpreempt].
+      exact (llcps_preempt_release Hlocal t c old j Hlt Hpreempt).
+Qed.
+
+Lemma local_labeled_concrete_projection_sound_current_not_completed :
+  forall CState (P : OSLabeledProjection CState) jobs m
+         (ex : labeled_concrete_execution P m),
+    local_labeled_concrete_projection_sound jobs m ex ->
+    forall t c j,
+      c < m ->
+      op_current
+        (os_to_op_state (osl_to_os_projection P) (lce_trace ex t))
+        c = Some j ->
+      ~ completed
+          jobs
+          m
+          (project_schedule (osl_to_op_trace P (lce_trace ex)))
+          j t.
+Proof.
+  intros CState P jobs m ex Hlocal.
+  induction t as [|t IH]; intros c j Hlt Hrun.
+  - exact (llcps_init_completion Hlocal c j Hlt Hrun).
+  - destruct (llcps_current_origin Hlocal t c j Hlt Hrun) as [Hprev | [Hdispatch | Hpreempt]].
+    + exact (llcps_persistent_completion Hlocal t c j Hlt Hprev Hrun).
+    + exact (llcps_dispatch_completion Hlocal t c j Hlt Hdispatch).
+    + destruct Hpreempt as [old Hpreempt].
+      exact (llcps_preempt_completion Hlocal t c old j Hlt Hpreempt).
+Qed.
+
+Lemma local_labeled_concrete_multicore_projection_sound_runnable_released :
+  forall CState (P : OSLabeledProjection CState) jobs adm m
+         (ex : labeled_concrete_execution P m),
+    local_labeled_concrete_multicore_projection_sound jobs adm m ex ->
+    forall t j,
+      In j
+         (op_runnable
+            (os_to_op_state (osl_to_os_projection P) (lce_trace ex t))) ->
+      released jobs j t.
+Proof.
+  intros CState P jobs adm m ex Hmulti.
+  induction t as [|t IH]; intros j Hin.
+  - exact (llcps_init_runnable_release (llcmps_projection_sound Hmulti) j Hin).
+  - pose proof (lce_stepwise ex t) as Hstep.
+    destruct (os_step_label P (lce_trace ex t) (lce_trace ex (S t))) eqn:Hev;
+      inversion Hstep; subst; clear Hstep;
+      repeat match goal with
+      | Hstate : _ = os_to_op_state (osl_to_os_projection P) (lce_trace ex (S t)) |- _ =>
+          rewrite <- Hstate in Hin
+      | Hstate : os_to_op_state (osl_to_os_projection P) (lce_trace ex (S t)) = _ |- _ =>
+          rewrite Hstate in Hin
+      end;
+      simpl in Hin.
+    + destruct Hin as [->|Hin].
+      * exact (llcps_wakeup_release (llcmps_projection_sound Hmulti) t j Hev).
+      * exact (released_monotone jobs j t (S t) (Nat.le_succ_diag_r t) (IH j Hin)).
+    + apply remove_job_in in Hin as [Hin _].
+      exact (released_monotone jobs j t (S t) (Nat.le_succ_diag_r t) (IH j Hin)).
+    + apply remove_job_in in Hin as [Hin _].
+      exact (released_monotone jobs j t (S t) (Nat.le_succ_diag_r t) (IH j Hin)).
+    + exact (released_monotone jobs j t (S t) (Nat.le_succ_diag_r t) (IH j Hin)).
+    + exact (released_monotone jobs j t (S t) (Nat.le_succ_diag_r t) (IH j Hin)).
+    + exact (released_monotone jobs j t (S t) (Nat.le_succ_diag_r t) (IH j Hin)).
+    + apply remove_job_in in Hin as [Hin _].
+      exact (released_monotone jobs j t (S t) (Nat.le_succ_diag_r t) (IH j Hin)).
+    + destruct Hin as [Heq|Hin].
+      * subst j.
+        assert (Hltc : c < m).
+        { destruct (lt_dec c m) as [Hltc|Hge]; auto.
+          assert (m <= c) by lia.
+          pose proof (llcmps_idle_outside Hmulti t c H) as Hid.
+          rewrite H4 in Hid.
+          discriminate. }
+        pose proof
+          (local_labeled_concrete_projection_sound_current_released
+             CState P jobs m ex (llcmps_projection_sound Hmulti) t c old Hltc H4) as Hrel_old.
+        exact (released_monotone jobs old t (S t) (Nat.le_succ_diag_r t) Hrel_old).
+      * apply remove_job_in in Hin as [Hin _].
+        exact (released_monotone jobs j t (S t) (Nat.le_succ_diag_r t) (IH j Hin)).
+    + exact (released_monotone jobs j t (S t) (Nat.le_succ_diag_r t) (IH j Hin)).
+    + exact (released_monotone jobs j t (S t) (Nat.le_succ_diag_r t) (IH j Hin)).
+Qed.
+
+Lemma local_labeled_concrete_multicore_projection_sound_runnable_not_completed :
+  forall CState (P : OSLabeledProjection CState) jobs adm m
+         (ex : labeled_concrete_execution P m),
+    local_labeled_concrete_multicore_projection_sound jobs adm m ex ->
+    forall t j,
+      In j
+         (op_runnable
+            (os_to_op_state (osl_to_os_projection P) (lce_trace ex t))) ->
+      ~ completed
+          jobs
+          m
+          (project_schedule (osl_to_op_trace P (lce_trace ex)))
+          j t.
+Proof.
+  intros CState P jobs adm m ex Hmulti.
+  induction t as [|t IH]; intros j Hin.
+  - exact (llcps_init_runnable_completion (llcmps_projection_sound Hmulti) j Hin).
+  - pose proof (lce_stepwise ex t) as Hstep.
+    pose proof (lce_struct_inv ex t) as Hinv.
+    destruct (os_step_label P (lce_trace ex t) (lce_trace ex (S t))) eqn:Hev;
+      inversion Hstep; subst; clear Hstep;
+      repeat match goal with
+      | Hstate : _ = os_to_op_state (osl_to_os_projection P) (lce_trace ex (S t)) |- _ =>
+          rewrite <- Hstate in Hin
+      | Hstate : os_to_op_state (osl_to_os_projection P) (lce_trace ex (S t)) = _ |- _ =>
+          rewrite Hstate in Hin
+      end;
+      simpl in Hin.
+    + destruct Hin as [->|Hin].
+      * exact (llcps_wakeup_completion (llcmps_projection_sound Hmulti) t j Hev).
+      * eapply visible_job_not_completed_if_not_running_next.
+        -- exact (IH j Hin).
+        -- eapply projected_trace_job_not_running_if_runnable; eauto.
+    + apply remove_job_in in Hin as [Hin _].
+      eapply visible_job_not_completed_if_not_running_next.
+      * exact (IH j Hin).
+      * eapply projected_trace_job_not_running_if_runnable; eauto.
+    + apply remove_job_in in Hin as [Hin _].
+      eapply visible_job_not_completed_if_not_running_next.
+      * exact (IH j Hin).
+      * eapply projected_trace_job_not_running_if_runnable; eauto.
+    + eapply visible_job_not_completed_if_not_running_next.
+      * exact (IH j Hin).
+      * eapply projected_trace_job_not_running_if_runnable; eauto.
+    + eapply visible_job_not_completed_if_not_running_next.
+      * exact (IH j Hin).
+      * eapply projected_trace_job_not_running_if_runnable; eauto.
+    + eapply visible_job_not_completed_if_not_running_next.
+      * exact (IH j Hin).
+      * eapply projected_trace_job_not_running_if_runnable; eauto.
+    + apply remove_job_in in Hin as [Hin _].
+      eapply visible_job_not_completed_if_not_running_next.
+      * exact (IH j Hin).
+      * eapply projected_trace_job_not_running_if_runnable; eauto.
+    + destruct Hin as [Heq|Hin].
+      * subst j.
+        assert (Hltc : c < m).
+        { destruct (lt_dec c m) as [Hltc|Hge]; auto.
+          assert (m <= c) by lia.
+          pose proof (llcmps_idle_outside Hmulti t c H) as Hid.
+          rewrite H4 in Hid.
+          discriminate. }
+        exact (llcps_preempt_old_completion (llcmps_projection_sound Hmulti) t c old new Hltc Hev).
+      * apply remove_job_in in Hin as [Hin _].
+        eapply visible_job_not_completed_if_not_running_next.
+        -- exact (IH j Hin).
+        -- eapply projected_trace_job_not_running_if_runnable; eauto.
+    + eapply visible_job_not_completed_if_not_running_next.
+      * exact (IH j Hin).
+      * eapply projected_trace_job_not_running_if_runnable; eauto.
+    + eapply visible_job_not_completed_if_not_running_next.
+      * exact (IH j Hin).
+      * eapply projected_trace_job_not_running_if_runnable; eauto.
+Qed.
+
+Lemma local_labeled_concrete_multicore_projection_sound_to_scheduler_view_contract :
+  forall CState (P : OSLabeledProjection CState) jobs adm m
+         (ex : labeled_concrete_execution P m),
+    local_labeled_concrete_multicore_projection_sound jobs adm m ex ->
+    labeled_concrete_scheduling_causality_contract jobs m ex ->
+    labeled_concrete_scheduler_view_contract jobs m ex.
+Proof.
+  intros CState P jobs adm m ex Hmulti Hcaus.
+  constructor.
+  - intros t j [[c [Hlt Hcur]] | [Hin | [c [Hlt Htarget]]]].
+    + eapply local_labeled_concrete_projection_sound_current_released; eauto.
+      exact (llcmps_projection_sound Hmulti).
+    + eapply local_labeled_concrete_multicore_projection_sound_runnable_released; eauto.
+    + pose proof (lce_struct_inv ex t) as Hinv.
+      destruct Hinv as [_ _ _ _ Hdispatch].
+      pose proof (Hdispatch c j Hlt Htarget) as Hin.
+      eapply local_labeled_concrete_multicore_projection_sound_runnable_released; eauto.
+  - intros t j [[c [Hlt Hcur]] | [Hin | [c [Hlt Htarget]]]].
+    + eapply local_labeled_concrete_projection_sound_current_not_completed; eauto.
+      exact (llcmps_projection_sound Hmulti).
+    + eapply local_labeled_concrete_multicore_projection_sound_runnable_not_completed; eauto.
+    + pose proof (lce_struct_inv ex t) as Hinv.
+      destruct Hinv as [_ _ _ _ Hdispatch].
+      pose proof (Hdispatch c j Hlt Htarget) as Hin.
+      eapply local_labeled_concrete_multicore_projection_sound_runnable_not_completed; eauto.
+  - intros t j Hwakeup.
+    right. left.
+    exact (lcsc_wakeup_visible Hcaus t j Hwakeup).
+  - intros t c j Hlt Hchoose.
+    right. right. exists c. split.
+    + exact Hlt.
+    + exact (lcsc_choose_sets_dispatch_target Hcaus t c j Hlt Hchoose).
+  - intros t c j Hlt Hdispatch.
+    left. exists c. split; [exact Hlt|].
+    exact (lcsc_dispatch_sets_current Hcaus t c j Hlt Hdispatch).
+  - intros t c old new Hlt Hpreempt.
+    right. left.
+    exact (lcsc_preempt_requeues_old Hcaus t c old new Hlt Hpreempt).
+  - intros t c old new Hlt Hpreempt.
+    left. exists c. split; [exact Hlt|].
+    exact (lcsc_preempt_sets_current Hcaus t c old new Hlt Hpreempt).
+  - intros t c j Hblock.
+    exact (llcps_block_clears_current (llcmps_projection_sound Hmulti) t c j Hblock).
+  - intros t j Hblock.
+    exact (llcps_block_clears_runnable (llcmps_projection_sound Hmulti) t j Hblock).
+  - intros t c j Hlt Hblock.
+    exact (llcps_block_clears_dispatch_target (llcmps_projection_sound Hmulti) t c j Hlt Hblock).
+  - intros t j Hcomplete.
+    exact (lcsc_complete_sets_completed Hcaus t j Hcomplete).
+  - intros t c j Hcomplete.
+    exact (lcsc_complete_clears_current Hcaus t c j Hcomplete).
+  - intros t j Hcomplete.
+    exact (lcsc_complete_clears_runnable Hcaus t j Hcomplete).
+  - intros t c j Hlt Hcomplete.
+    exact (lcsc_complete_clears_dispatch_target Hcaus t c j Hlt Hcomplete).
+Qed.
+
+Definition os_local_scheduler_view_contract
+    {CState : Type}
+    {P : OSLabeledProjection CState}
+    {jobs : JobId -> Job}
+    {adm : admissible_cpu}
+    {m : nat}
+    (C : os_local_multicore_adapter_contract P jobs adm m) : Prop :=
+  labeled_concrete_scheduler_view_contract jobs m (olac_execution C).
+
+Lemma os_local_multicore_adapter_contract_to_scheduler_view_contract :
+  forall CState (P : OSLabeledProjection CState) jobs adm m
+         (C : os_local_multicore_adapter_contract P jobs adm m),
+    os_local_scheduler_view_contract C.
+Proof.
+  intros CState P jobs adm m C.
+  unfold os_local_scheduler_view_contract.
+  eapply local_labeled_concrete_multicore_projection_sound_to_scheduler_view_contract.
+  - exact (olac_sound C).
+  - apply os_local_multicore_adapter_contract_to_causality_contract.
+Qed.
